theories/Classes/Relations.v
@@ -7,11 +7,11 @@
 (*         *       GNU Lesser General Public License Version 2.1        *)
 (************************************************************************)
 
-(* Typeclass-based setoids, tactics and standard instances.
-   TODO: explain clrewrite, clsubstitute and so on.
+(* Typeclass-based relations, tactics and standard instances.
+   This is the basic theory needed to formalize morphisms and setoids.
  
    Author: Matthieu Sozeau
-   Institution: LRI, CNRS UMR 8623 - UniversitÃƒcopyright Paris Sud
+   Institution: LRI, CNRS UMR 8623 - UniversitÃcopyright Paris Sud
    91405 Orsay, France *)
 
 (* $Id: FSetAVL_prog.v 616 2007-08-08 12:28:10Z msozeau $ *)
@@ -25,14 +25,14 @@ Unset Strict Implicit.
 Definition relationT A := A -> A -> Type.
 Definition relation A := A -> A -> Prop.
 
-Definition inverse A (R : relation A) : relation A := flip R.
+Definition inverse A (R : relation A) : relation A := fun x y => R y x.
 
 Lemma inverse_inverse : forall A (R : relation A), inverse (inverse R) = R.
 Proof. intros ; unfold inverse. apply (flip_flip R). Qed.
 
-Definition complementT A (R : relationT A) := fun x y => ! R x y.
+Definition complementT A (R : relationT A) := fun x y => notT (R x y).
 
-Definition complement A (R : relation A) := fun x y => ~ R x y.
+Definition complement A (R : relation A) := fun x y => R x y -> False.
 
 (** These are convertible. *)
 
@@ -112,7 +112,6 @@ Program Instance [ Reflexive A (R : relation A) ] =>
 
   Next Obligation. 
   Proof. 
-    unfold complement in * ; intros.
     apply H.
     apply reflexive.
   Qed.
@@ -122,7 +121,6 @@ Program Instance [ Irreflexive A (R : relation A) ] =>
 
   Next Obligation. 
   Proof. 
-    unfold complement in * ; intros.
     red ; intros.
     apply (irreflexive H).
   Qed.
@@ -131,12 +129,54 @@ Program Instance [ Symmetric A (R : relation A) ] => complement_symmetric : Symm
 
   Next Obligation.
   Proof.
-    unfold complement in *.
     red ; intros H'.
     apply (H (symmetric H')).
   Qed.
 
-(** Tactics to solve goals. Each tactic comes in two flavors:
+(** * Standard instances. *)
+
+Ltac simpl_relation :=
+  try red ; unfold inverse, flip, impl, arrow ; program_simpl ; try tauto ; 
+    repeat (red ; intros) ; try ( solve [ intuition ]).
+
+Ltac obligations_tactic ::= simpl_relation.
+
+(** The arrow is a reflexive and transitive relation on types. *)
+
+Program Instance arrow_refl : ? Reflexive arrow := 
+  reflexive X := id.
+
+Program Instance arrow_trans : ? Transitive arrow := 
+  transitive X Y Z f g := g o f.
+
+(** Isomorphism. *)
+
+Definition iso (A B : Type) := 
+  A -> B * B -> A.
+
+Program Instance iso_refl : ? Reflexive iso.
+Program Instance iso_sym : ? Symmetric iso.
+Program Instance iso_trans : ? Transitive iso.
+
+(** Logical implication. *)
+
+Program Instance impl_refl : ? Reflexive impl.
+Program Instance impl_trans : ? Transitive impl.
+
+(** Logical equivalence. *)
+
+Program Instance iff_refl : ? Reflexive iff.
+Program Instance iff_sym : ? Symmetric iff.
+Program Instance iff_trans : ? Transitive iff.
+
+(** Leibniz equality. *)
+
+Program Instance eq_refl : ? Reflexive (@eq A).
+Program Instance eq_sym : ? Symmetric (@eq A).
+Program Instance eq_trans : ? Transitive (@eq A).
+
+(** ** General tactics to solve goals on relations.
+   Each tactic comes in two flavors:
    - a tactic to immediately solve a goal without user intervention
    - a tactic taking input from the user to make progress on a goal *)
 
@@ -216,6 +256,9 @@ Ltac relation_trans :=
 
     | [ H : ?R ?A ?B ?C ?D ?X ?Y, H' : ?R ?A ?B ?C ?D ?Y ?Z |- ?R ?A ?B ?C ?D ?X ?Z ] => 
       apply (transitive (R:=R A B C D) (x:=X) (y:=Y) (z:=Z) H H')
+
+    | [ H : ?R ?A ?B ?C ?D ?E ?X ?Y, H' : ?R ?A ?B ?C ?D ?E ?Y ?Z |- ?R ?A ?B ?C ?D ?E ?X ?Z ] => 
+      apply (transitive (R:=R A B C D E) (x:=X) (y:=Y) (z:=Z) H H')
   end.
 
 Ltac relation_transitive Y := 
@@ -242,254 +285,13 @@ Ltac trans Y := relation_transitive Y.
 
 Ltac relation_tac := relation_refl || relation_sym || relation_trans.
 
-(** * Morphisms.
-
-   We now turn to the definition of [Morphism] and declare standard instances. 
-   These will be used by the [clrewrite] tactic later. *)
-
-(** Respectful morphisms. *)
-
-Definition respectful_depT (A : Type) (R : relationT A) 
-  (B : A -> Type) (R' : forall x y, B x -> B y -> Type) : relationT (forall x : A, B x) := 
-  fun f g => forall x y : A, R x y -> R' x y (f x) (g y).
-
-Definition respectfulT A (eqa : relationT A) B (eqb : relationT B) : relationT (A -> B) :=
-  Eval compute in (respectful_depT eqa (fun _ _ => eqb)).
-
-Definition respectful A (R : relation A) B (R' : relation B) : relation (A -> B) :=
-  fun f g => forall x y : A, R x y -> R' (f x) (g y).
-
-(** Notations reminiscent of the old syntax for declaring morphisms.
-   We use three + or - for type morphisms, and two for [Prop] ones.
-   *)
-
-Notation " R +++> R' " := (@respectfulT _ R _ R') (right associativity, at level 20).
-Notation " R ---> R' " := (@respectfulT _ (flip R) _ R') (right associativity, at level 20).
-
-Notation " R ++> R' " := (@respectful _ R _ R') (right associativity, at level 20).
-Notation " R --> R' " := (@respectful _ (inverse R) _ R') (right associativity, at level 20).
-
-(** A morphism on a relation [R] is an object respecting the relation (in its kernel). 
-   The relation [R] will be instantiated by [respectful] and [A] by an arrow type 
-   for usual morphisms. *)
-
-Class Morphism A (R : relationT A) (m : A) :=
-  respect : R m m.
-
-Ltac simpl_morphism :=
-  try red ; unfold inverse, flip, impl, arrow ; program_simpl ; try tauto ; 
-    try (red ; intros) ; try ( solve [ intuition ]).
-
-Ltac obligations_tactic ::= simpl_morphism.
-
-(** The arrow is a reflexive and transitive relation on types. *)
-
-Program Instance arrow_refl : ? Reflexive arrow := 
-  reflexive X := id.
-
-Program Instance arrow_trans : ? Transitive arrow := 
-  transitive X Y Z f g := g o f.
-
-(** Can't use the definition [notT] as it gives a to universe inconsistency. *)
-
-Program Instance notT_arrow_morphism : 
-  Morphism (Type -> Type) (arrow ---> arrow) (fun X : Type => X -> False).
-
-(** Isomorphism. *)
-
-Definition iso (A B : Type) := 
-  A -> B * B -> A.
-
-Program Instance iso_refl : ? Reflexive iso.
-Program Instance iso_sym : ? Symmetric iso.
-Program Instance iso_trans : ? Transitive iso.
-
-Program Instance not_iso_morphism : 
-  Morphism (Type -> Type) (iso +++> iso) (fun X : Type => X -> False).
-
-(** Logical implication. *)
-
-Program Instance impl_refl : ? Reflexive impl.
-Program Instance impl_trans : ? Transitive impl.
-
-Program Instance not_impl_morphism :
-  Morphism (Prop -> Prop) (impl --> impl) not.
-
-(** Logical equivalence. *)
-
-Program Instance iff_refl : ? Reflexive iff.
-Program Instance iff_sym : ? Symmetric iff.
-Program Instance iff_trans : ? Transitive iff.
-
-Program Instance not_iff_morphism : 
-  Morphism (Prop -> Prop) (iff ++> iff) not.
-
-(** We make the type implicit, it can be infered from the relations. *)
-
-Implicit Arguments Morphism [A].
-
-(** If you have a morphism from [RA] to [RB] you have a contravariant morphism 
-   from [RA] to [inverse RB]. *)
-
-Program Instance `A` (RA : relation A) `B` (RB : relation B) [ ? Morphism (RA ++> RB) m ] =>
-  morph_impl_co_contra_inverse :
-  ? Morphism (RA --> inverse RB) m.
-
-  Next Obligation.
-  Proof.
-    apply respect.
-    apply H.
-  Qed.
-
-(** Every transitive relation gives rise to a binary morphism on [impl], 
-   contravariant in the first argument, covariant in the second. *)
-
-Program Instance [ Transitive A (R : relation A) ] => 
-  trans_contra_co_morphism : ? Morphism (R --> R ++> impl) R.
-
-  Next Obligation.
-  Proof with auto.
-    trans x...
-    trans x0...
-  Qed.
-
-(** Dually... *)
-
-Program Instance [ Transitive A (R : relation A) ] =>
-  trans_co_contra_inv_impl_morphism : ? Morphism (R ++> R --> inverse impl) R.
-
-  Obligations Tactic := idtac.
-  
-  Next Obligation.
-  Proof with auto.
-    intros.
-    destruct (trans_contra_co_morphism (R:=inverse R)).
-    revert respect0.
-    unfold respectful, inverse, flip in * ; intros.
-    apply respect0 ; auto.
-  Qed.
-
-Obligations Tactic := simpl_morphism.
-
-(** With symmetric relations, variance is no issue ! *)
-
-Program Instance [ Symmetric A (R : relation A) ] B (R' : relation B) 
-  [ Morphism _ (R ++> R') m ] => 
-  sym_contra_morphism : ? Morphism (R --> R') m.
-
-  Next Obligation.
-  Proof with auto.
-    apply respect.
-    sym...
-  Qed.
-
-(** Every symmetric and transitive relation gives rise to an equivariant morphism. *)
-
-Program Instance [ Transitive A (R : relation A), Symmetric A R ] => 
-  trans_sym_morphism : ? Morphism (R ++> R ++> iff) R.
-
-  Next Obligation.
-  Proof with auto.
-    split ; intros.
-    trans x0... trans x... sym...
-  
-    trans y... trans y0... sym...
-  Qed.
-
-(** The complement of a relation conserves its morphisms. *)
-
-Program Instance `A` (RA : relation A) [ ? Morphism (RA ++> RA ++> iff) R ] => 
-  complement_morphism : ? Morphism (RA ++> RA ++> iff) (complement R).
-
-  Next Obligation.
-  Proof.
-    red ; unfold complement ; intros.
-    pose (respect).
-    pose (r x y H).
-    pose (r0 x0 y0 H0).
-    intuition.
-  Qed.
-
-(** The inverse too. *)
-
-Program Instance `A` (RA : relation A) [ ? Morphism (RA ++> RA ++> iff) R ] => 
-  inverse_morphism : ? Morphism (RA ++> RA ++> iff) (inverse R).
-
-  Next Obligation.
-  Proof.
-    unfold inverse ; unfold flip.
-    apply respect ; auto.
-  Qed.
-
-Program Instance [ Transitive A (R : relation A), Symmetric A R ] =>
-  trans_sym_contra_co_inv_impl_morphism : ? Morphism (R --> R ++> inverse impl) R.
-
-  Next Obligation.
-  Proof with auto.
-    trans y...
-    sym...
-    trans y0...
-    sym...
-  Qed.
-
-(** Any binary morphism respecting some relations up to [iff] respects 
-   them up to [impl] in each way. Very important instances as we need [impl]
-   morphisms at the top level when we rewrite. *)
-
-Program Instance `A` (R : relation A) `B` (R' : relation B) 
-  [ ? Morphism (R ++> R' ++> iff) m ] => 
-  iff_impl_binary_morphism : ? Morphism (R ++> R' ++> impl) m.
-
-  Next Obligation.
-  Proof.
-    destruct respect with x y x0 y0 ; auto.
-  Qed.
-
-Program Instance `A` (R : relation A) `B` (R' : relation B)
-  [ ? Morphism (R ++> R' ++> iff) m ] => 
-  iff_inverse_impl_binary_morphism : ? Morphism (R ++> R' ++> inverse impl) m.
-
-  Next Obligation.
-  Proof.
-    destruct respect with x y x0 y0 ; auto.
-  Qed.
-
-(** Standard instances for [iff] and [impl]. *)
-
-(** Logical conjunction. *)
-
-Program Instance and_impl_iff_morphism : ? Morphism (impl ++> iff ++> impl) and.
-
-Program Instance and_iff_impl_morphism : ? Morphism (iff ++> impl ++> impl) and.
-
-Program Instance and_iff_morphism : ? Morphism (iff ++> iff ++> iff) and.
-
-(** Logical disjunction. *)
-
-Program Instance or_impl_iff_morphism : ? Morphism (impl ++> iff ++> impl) or.
-
-Program Instance or_iff_impl_morphism : ? Morphism (iff ++> impl ++> impl) or.
-
-Program Instance or_iff_morphism : ? Morphism (iff ++> iff ++> iff) or.
-
-(** Leibniz equality. *)
-
-Program Instance eq_refl : ? Reflexive (@eq A).
-Program Instance eq_sym : ? Symmetric (@eq A).
-Program Instance eq_trans : ? Transitive (@eq A).
-
-Program Definition eq_morphism A : Morphism (eq ++> eq ++> iff) (eq (A:=A)) :=
-  trans_sym_morphism.
-
-Program Instance `A B` (m : A -> B) => arrow_morphism : ? Morphism (eq ++> eq) m.
-
 (** The [PER] typeclass. *)
 
 Class PER (carrier : Type) (pequiv : relationT carrier) :=
   per_sym :> Symmetric pequiv ;
   per_trans :> Transitive pequiv.
 
-(** We can build a PER on the coq function space if we have PERs on the domain and
+(** We can build a PER on the Coq function space if we have PERs on the domain and
    codomain. *)
 
 Program Instance [ PER A (R : relation A), PER B (R' : relation B) ] => 
@@ -520,38 +322,10 @@ Program Instance [ eq : Equivalence A eqA, ? Antisymmetric eq R ] =>
 
   Solve Obligations using unfold flip ; program_simpl ; eapply antisymmetric ; eauto.
 
-(** Here we build an equivalence instance for functions which relates respectful ones only. *)
+Program Instance [ eq : Equivalence A eqA, ? Antisymmetric eq (R : relation A) ] => 
+  inverse_antisymmetric : ? Antisymmetric eq (inverse R).
 
-Definition respecting [ Equivalence A (R : relation A), Equivalence B (R' : relation B) ] : Type := 
-  { morph : A -> B | respectful R R' morph morph }.
-
-Ltac obligations_tactic ::= program_simpl.
-
-Program Instance [ Equivalence A (R : relation A), Equivalence B (R' : relation B) ] => 
-  respecting_equiv : Equivalence respecting
-  (fun (f g : respecting) => forall (x y : A), R x y -> R' (`f x) (`g y)).
-
-  Next Obligation.
-  Proof.
-    constructor ; intros.
-    destruct x ; simpl.
-    apply r ; auto.
-  Qed.
-
-  Next Obligation.
-  Proof.
-    constructor ; intros.
-    sym ; apply H.
-    sym ; auto.
-  Qed.
-
-  Next Obligation.
-  Proof.
-    constructor ; intros.
-    trans ((`y) y0).
-    apply H ; auto.
-    apply H0. refl.
-  Qed.
+  Solve Obligations using unfold inverse, flip ; program_simpl ; eapply antisymmetric ; eauto.
 
 (** Leibinz equality [eq] is an equivalence relation. *)
 
