theories/Classes/Init.v
@@ -1,1 +1,1 @@
-Ltac typeclass_instantiation := eauto 50 with typeclass_instances || eauto.
+Ltac typeclass_instantiation := eauto with typeclass_instances || eauto.
