theories/Classes/Morphisms.v
@@ -1,0 +1,350 @@
+(* -*- coq-prog-args: ("-emacs-U" "-nois") -*- *)
+(************************************************************************)
+(*  v      *   The Coq Proof Assistant  /  The Coq Development Team     *)
+(* <O___,, * CNRS-Ecole Polytechnique-INRIA Futurs-Universite Paris Sud *)
+(*   \VV/  **************************************************************)
+(*    //   *      This file is distributed under the terms of the       *)
+(*         *       GNU Lesser General Public License Version 2.1        *)
+(************************************************************************)
+
+(* Typeclass-based morphisms with standard instances for equivalence relations.
+ 
+   Author: Matthieu Sozeau
+   Institution: LRI, CNRS UMR 8623 - UniversitÃcopyright Paris Sud
+   91405 Orsay, France *)
+
+(* $Id: FSetAVL_prog.v 616 2007-08-08 12:28:10Z msozeau $ *)
+
+Require Import Coq.Program.Program.
+Require Import Coq.Classes.Init.
+Require Export Coq.Classes.Relations.
+
+Set Implicit Arguments.
+Unset Strict Implicit.
+
+(** * Morphisms.
+
+   We now turn to the definition of [Morphism] and declare standard instances. 
+   These will be used by the [clrewrite] tactic later. *)
+
+(** Respectful morphisms. *)
+
+Definition respectful_depT (A : Type) (R : relationT A) 
+  (B : A -> Type) (R' : forall x y, B x -> B y -> Type) : relationT (forall x : A, B x) := 
+  fun f g => forall x y : A, R x y -> R' x y (f x) (g y).
+
+Definition respectfulT A (eqa : relationT A) B (eqb : relationT B) : relationT (A -> B) :=
+  Eval compute in (respectful_depT eqa (fun _ _ => eqb)).
+
+Definition respectful A (R : relation A) B (R' : relation B) : relation (A -> B) :=
+  fun f g => forall x y : A, R x y -> R' (f x) (g y).
+
+(** Notations reminiscent of the old syntax for declaring morphisms.
+   We use three + or - for type morphisms, and two for [Prop] ones.
+   *)
+
+Notation " R +++> R' " := (@respectfulT _ R _ R') (right associativity, at level 20).
+Notation " R ---> R' " := (@respectfulT _ (flip R) _ R') (right associativity, at level 20).
+
+Notation " R ++> R' " := (@respectful _ R _ R') (right associativity, at level 20).
+Notation " R --> R' " := (@respectful _ (inverse R) _ R') (right associativity, at level 20).
+
+(** A morphism on a relation [R] is an object respecting the relation (in its kernel). 
+   The relation [R] will be instantiated by [respectful] and [A] by an arrow type 
+   for usual morphisms. *)
+
+Class Morphism A (R : relationT A) (m : A) :=
+  respect : R m m.
+
+(** Here we build an equivalence instance for functions which relates respectful ones only. *)
+
+Definition respecting [ Equivalence A (R : relation A), Equivalence B (R' : relation B) ] : Type := 
+  { morph : A -> B | respectful R R' morph morph }.
+
+Ltac obligations_tactic ::= program_simpl.
+
+Program Instance [ Equivalence A (R : relation A), Equivalence B (R' : relation B) ] => 
+  respecting_equiv : Equivalence respecting
+  (fun (f g : respecting) => forall (x y : A), R x y -> R' (`f x) (`g y)).
+
+  Next Obligation.
+  Proof.
+    constructor ; intros.
+    destruct x ; simpl.
+    apply r ; auto.
+  Qed.
+
+  Next Obligation.
+  Proof.
+    constructor ; intros.
+    sym ; apply H.
+    sym ; auto.
+  Qed.
+
+  Next Obligation.
+  Proof.
+    constructor ; intros.
+    trans ((`y) y0).
+    apply H ; auto.
+    apply H0. refl.
+  Qed.
+
+(** Can't use the definition [notT] as it gives a universe inconsistency. *)
+
+Ltac obligations_tactic ::= program_simpl ; simpl_relation.
+
+Program Instance notT_arrow_morphism : 
+  Morphism (Type -> Type) (arrow ---> arrow) (fun X : Type => X -> False).
+
+Program Instance not_iso_morphism : 
+  Morphism (Type -> Type) (iso +++> iso) (fun X : Type => X -> False).
+
+Program Instance not_impl_morphism :
+  Morphism (Prop -> Prop) (impl --> impl) not.
+
+Program Instance not_iff_morphism : 
+  Morphism (Prop -> Prop) (iff ++> iff) not.
+
+(** We make the type implicit, it can be infered from the relations. *)
+
+Implicit Arguments Morphism [A].
+
+(** Leibniz *)
+
+Program Definition eq_morphism A : Morphism (eq ++> eq ++> iff) (eq (A:=A)).
+Proof. intros ; constructor ; intros.
+  obligations_tactic.
+  subst.
+  intuition.
+Qed.
+
+(* Program Definition arrow_morphism `A B` (m : A -> B) : Morphism (eq ++> eq) m. *)
+
+(** Any binary morphism respecting some relations up to [iff] respects 
+   them up to [impl] in each way. Very important instances as we need [impl]
+   morphisms at the top level when we rewrite. *)
+
+Program Instance `A` (R : relation A) `B` (R' : relation B)
+  [ ? Morphism (R ++> R' ++> iff) m ] =>
+
+  iff_impl_binary_morphism : ? Morphism (R ++> R' ++> impl) m.
+
+  Next Obligation.
+  Proof.
+    destruct respect with x y x0 y0 ; auto.
+  Qed.
+
+Program Instance `A` (R : relation A) `B` (R' : relation B)
+  [ ? Morphism (R ++> R' ++> iff) m ] =>
+  iff_inverse_impl_binary_morphism : ? Morphism (R ++> R' ++> inverse impl) m.
+
+  Next Obligation.
+  Proof.
+    destruct respect with x y x0 y0 ; auto.
+  Qed.
+
+(** The complement of a relation conserves its morphisms. *)
+
+Program Instance `A` (RA : relation A) [ ? Morphism (RA ++> RA ++> iff) R ] => 
+  complement_morphism : ? Morphism (RA ++> RA ++> iff) (complement R).
+
+  Next Obligation.
+  Proof.
+    unfold complement ; intros.
+    pose (respect).
+    pose (r x y H).
+    pose (r0 x0 y0 H0).
+    intuition.
+  Qed.
+
+(** The inverse too. *)
+
+Program Instance `A` (RA : relation A) [ ? Morphism (RA ++> RA ++> iff) R ] => 
+  inverse_morphism : ? Morphism (RA ++> RA ++> iff) (inverse R).
+
+  Next Obligation.
+  Proof.
+    unfold inverse ; unfold flip.
+    apply respect ; auto.
+  Qed.
+
+(* Definition respectful' A (R : relation A) B (R' : relation B) (f : A -> B) : relation A := *)
+(*   fun x y => R x y -> R' (f x) (f y). *)
+
+(* Definition morphism_respectful' A (R : relation A) B (R' : relation B) (f : A -> B) *)
+(*   [ ? Morphism (R ++> R') f ] (x y : A) : respectful' R R' f x y. *)
+(* intros. *)
+(* destruct H. *)
+(* red in respect0. *)
+(* red.  *)
+(* apply respect0. *)
+(* Qed. *)
+
+(* Existing Instance morphism_respectful'. *)
+
+(* Goal forall A [ Equivalence A (eqA : relation A) ] (R : relation A) [ ? Morphism (eqA ++> iff) m ] (x y : A)  *)
+(*   [ ? Morphism (eqA ++> eqA) m' ] (m' : A -> A), eqA x y -> True. *)
+(*   intros. *)
+(*   cut (relation A) ; intros R'. *)
+(*   cut ((eqA ++> R') m' m') ; intros. *)
+(*   assert({ R' : relation A & Reflexive R' }). *)
+(*   econstructor. *)
+(*   typeclass_instantiation. *)
+  
+
+(*   assert (exists R' : relation A, Morphism ((fun x y => eqA x y -> R' (m' x) (m' y)) ++> iff) m). *)
+(*   eapply ex_intro. *)
+(*   unfold respectful. *)
+(*   typeclass_instantiation. *)
+  
+
+(*   assert (exists R', Morphism (R' ++> iff) m /\ Morphism (eqA ++> R') m'). *)
+(*   typeclass_instantiation. *)
+(*   Set Printing All. *)
+(*   Show Proof. *)
+  
+  
+(*   apply respect. *)
+
+(** Partial applications are ok when a proof of refl is available. *)
+
+(** A proof of [R x x] is available. *)
+
+(* Program Instance (A : Type) (R : relation A) B (R' : relation B) *)
+(*   [ ? Morphism (R ++> R') m ] [ ? Morphism R x ] => *)
+(*   morphism_partial_app_morphism : ? Morphism R' (m x). *)
+
+(*   Next Obligation. *)
+(*   Proof with auto. *)
+(*     apply (respect (m:=m))... *)
+(*     apply respect. *)
+(*   Qed. *)
+
+
+(** Morpshism declarations for partial applications. *)
+
+Program Instance [ Transitive A (R : relation A) ] (x : A) =>
+  trans_contra_inv_impl_morphism : ? Morphism (R --> inverse impl) (R x).
+
+  Next Obligation.
+  Proof with auto.
+    trans y...
+  Qed.
+
+Program Instance [ Transitive A (R : relation A) ] (x : A) =>
+  trans_co_impl_morphism : ? Morphism (R ++> impl) (R x).
+
+  Next Obligation.
+  Proof with auto.
+    trans x0...
+  Qed.
+
+Program Instance [ Transitive A (R : relation A), Symmetric A R ] (x : A) =>
+  trans_sym_co_inv_impl_morphism : ? Morphism (R ++> inverse impl) (R x).
+
+  Next Obligation.
+  Proof with auto.
+    trans y...
+    sym...
+  Qed.
+
+Program Instance [ Transitive A (R : relation A), Symmetric A R ] (x : A) =>
+  trans_sym_contra_impl_morphism : ? Morphism (R --> impl) (R x).
+
+  Next Obligation.
+  Proof with auto.
+    trans x0...
+    sym...
+  Qed.
+
+Program Instance [ Equivalence A (R : relation A) ] (x : A) =>
+  equivalence_partial_app_morphism : ? Morphism (R ++> iff) (R x).
+
+  Next Obligation.
+  Proof with auto.
+    split. intros ; trans x0...
+    intros.
+    trans y...
+    sym...
+  Qed.
+
+(** With symmetric relations, variance is no issue ! *)
+
+Program Instance [ Symmetric A (R : relation A) ] B (R' : relation B) 
+  [ Morphism _ (R ++> R') m ] => 
+  sym_contra_morphism : ? Morphism (R --> R') m.
+
+  Next Obligation.
+  Proof with auto.
+    repeat (red ; intros). apply respect.
+    sym...
+  Qed.
+
+(** [R] is reflexive, hence we can build the needed proof. *)
+
+Program Instance [ Reflexive A (R : relation A) ] B (R' : relation B)
+  [ ? Morphism (R ++> R') m ] (x : A) =>
+  reflexive_partial_app_morphism : ? Morphism R' (m x).
+
+  Next Obligation.
+  Proof with auto.
+    intros.
+    apply (respect (m:=m))...
+    refl.
+  Qed.
+
+(** Every symmetric and transitive relation gives rise to an equivariant morphism. *)
+
+Program Instance [ Transitive A (R : relation A), Symmetric A R ] => 
+  trans_sym_morphism : ? Morphism (R ++> R ++> iff) R.
+
+  Next Obligation.
+  Proof with auto.
+    split ; intros.
+    trans x0... trans x... sym...
+  
+    trans y... trans y0... sym...
+  Qed.
+
+Program Instance [ Equivalence A (R : relation A) ] => 
+  equiv_morphism : ? Morphism (R ++> R ++> iff) R.
+
+  Next Obligation.
+  Proof with auto.
+    split ; intros.
+    trans x0... trans x... sym...
+  
+    trans y... trans y0... sym...
+  Qed.
+
+(** In case the rewrite happens at top level. *)
+
+Program Instance iff_inverse_impl_id : 
+  ? Morphism (iff ++> inverse impl) id.
+
+Program Instance inverse_iff_inverse_impl_id : 
+  ? Morphism (iff --> inverse impl) id.
+  
+Program Instance iff_impl_id : 
+  ? Morphism (iff ++> impl) id.
+
+Program Instance inverse_iff_impl_id : 
+  ? Morphism (iff --> impl) id.
+  
+(** Standard instances for [iff] and [impl]. *)
+
+(** Logical conjunction. *)
+
+(* Program Instance and_impl_iff_morphism : ? Morphism (impl ++> iff ++> impl) and. *)
+
+(* Program Instance and_iff_impl_morphism : ? Morphism (iff ++> impl ++> impl) and. *)
+
+Program Instance and_iff_morphism : ? Morphism (iff ++> iff ++> iff) and.
+
+(** Logical disjunction. *)
+
+(* Program Instance or_impl_iff_morphism : ? Morphism (impl ++> iff ++> impl) or. *)
+
+(* Program Instance or_iff_impl_morphism : ? Morphism (iff ++> impl ++> impl) or. *)
+
+Program Instance or_iff_morphism : ? Morphism (iff ++> iff ++> iff) or.
